Progress made with Ale

semantics/proofs/chorIforestPropsScript.sml
@@ -439,32 +439,37 @@ End
 
 Inductive to_chor_forest:
 [~init:]
-  (∀c s. to_chor_forest c (chor_iforest c s)) ∧
+  (∀c s.
+     to_chor_forest (chor_iforest c s)) ∧
 [~step:]
-  (∀c p.
-     MEM p (procsOf c) ∧ iforest_can_act ψ p ∧
-     (∀p. p ∈ iforest_itrees ψ ⇒ to_chor_forest c (iforest_step ψ p)) ⇒
-     to_chor_forest c ψ)
+  (∀p ψ.
+     iforest_can_act ψ p ∧
+     (∀p. iforest_can_act ψ p ⇒ to_chor_forest (iforest_step ψ p)) ⇒
+     to_chor_forest ψ)
 End
 
 Theorem iforest_step_to_chor_forest:
   ∀c s p.
     MEM p (procsOf c) ⇒
-    to_chor_forest c (iforest_step (chor_iforest c s) p)
+    to_chor_forest (iforest_step (chor_iforest c s) p)
+Proof
+  cheat
+QED
+
+Theorem iforest_step_skip:
+  ¬iforest_can_act ψ p ⇒ iforest_step ψ p = ψ
 Proof
   cheat
 QED
 
 Theorem iforest_step_preserves_to_chor_forest:
-  ∀c ψ. to_chor_forest c ψ ⇒ to_chor_forest c (iforest_step ψ p)
+  ∀ψ. to_chor_forest ψ ⇒ to_chor_forest (iforest_step ψ p)
 Proof
   rw[]
   \\ first_assum mp_tac
   \\ simp_tac std_ss [Once to_chor_forest_cases] \\ reverse (rw[])
-  >- (Cases_on ‘p ∈ iforest_itrees ψ’
-      >- metis_tac []
-      >- (gs[iforest_itrees_def]
-          \\ rw[iforest_step_def,iforest_get_def,FLOOKUP_DEF]))
+  >- (Cases_on ‘iforest_can_act ψ p’
+      \\ metis_tac [iforest_step_skip])
   >- (Cases_on ‘p ∈ iforest_itrees (chor_iforest c s)’
       >- fs[iforest_step_to_chor_forest,chor_iforest_itrees_eq_procOf]
       >- (iforest_simp \\ simp[FLOOKUP_DEF]))
@@ -474,22 +479,26 @@ Theorem iforest_steps_IMP_Res:
   ∀f s res.
     iforest_steps f s res ⇒
     ∀c p.
-      set (procsOf c) ⊆ s ∧ to_chor_forest c f ∧ MEM p (procsOf c) ⇒
+      s = UNIV ∧ to_chor_forest f ∧ p ∈ iforest_itrees f ⇒
       EXISTS (λ(q,a). p = q ∧ ∃t. a = Res t) res
 Proof
   Induct_on ‘iforest_steps’ \\ rpt strip_tac
   >- (gvs [SUBSET_DEF]
-      \\ fs [Once to_chor_forest_cases]
-      >- metis_tac [iforest_can_act_exists]
-      \\ metis_tac [])
+      \\ fs [Once to_chor_forest_cases] \\ gvs []
+      \\ gvs [chor_iforest_itrees_eq_procOf]
+      \\ metis_tac [iforest_can_act_exists])
   \\ gvs []
   \\ rewrite_tac [METIS_PROVE [] “b ∨ c ⇔ ~b ⇒ c”]
   \\ strip_tac
   \\ first_x_assum irule
-  \\ irule_at Any SUBSET_TRANS
-  \\ first_x_assum $ irule_at $ Pos $ el 2
   \\ irule_at Any iforest_step_preserves_to_chor_forest
-  \\ first_x_assum $ irule_at $ Pos hd \\ fs []
+  \\ fs []
+  \\ pairarg_tac \\ fs []
+  \\ iforest_simp \\ fs [FLOOKUP_DEF]
+  \\ Cases_on ‘p' = q’ \\ gvs []
+  \\ every_case_tac \\ gvs [iforest_get_def,FLOOKUP_DEF]
+  \\ CCONTR_TAC \\ gvs []
+  \\ gvs [iforest_act_def,iforest_get_def,FLOOKUP_DEF]
 QED
 
 Theorem chor_iforest_deadlock_freedom:
@@ -500,13 +509,15 @@ Proof
   simp [deadlock_freedom_def]
   \\ rpt gen_tac \\ strip_tac
   \\ conj_asm1_tac
-  >- cheat (* actions_end (iforest (chor_iforest ...)) *)
+  >- simp [iforestTheory.actions_end_iforest]
   \\ CCONTR_TAC \\ fs []
   \\ drule_all LFINITE_iforest
   \\ strip_tac \\ fs [exists_fromList]
   \\ drule iforest_steps_IMP_Res \\ simp []
   \\ irule_at Any to_chor_forest_init
   \\ first_x_assum $ irule_at Any \\ fs []
+  \\ fs [chor_iforest_itrees_eq_procOf]
+  \\ cheat
 QED
 
 Theorem chor_iforest_always_rooted:
